\documentclass{article}
%\usepackage{amssymbol}

\setlength{\parindent}{0pt} 
\def\therefore{%
     \leavevmode
     \lower0.2ex\hbox{$\circ$}%
     \kern-0.2em\raise0.7ex\hbox{$\circ$}%
     \kern-0.2em\lower0.2ex\hbox{$\circ$}%
     \thinspace}

\begin{document}
Definition 1: $\cdot$ (and)
\begin{itemize}
\item
$p$

$q$

$\therefore p \cdot q$
\item
$p \cdot q$

$\therefore p$

$\therefore q$

\end{itemize}
\\
Definition 2: $\vee$ (or)

\begin{itemize}
\item
$p \vee q$

$\sim p$

$\therefore q$

\item
$p$

$p \vee q$


\end{itemize}

\\
Definition 3: $\rightarrow$ (if-then)

$p \rightarrow q$

$p$

$\therefore q$
\\
Theorem 1: (commutativity of $\cdot$)

$p \cdot q$

$p$

$q$

$\therefore q \cdot p$
\\
Exercise 1:

Prove that $p \vee q \rightarrow q \vee p$.
(We denote this property by saying that $\vee$ is commutative.)

Theorem 2: (De Morgan)

$\sim (p \vee q)$

\indent $p$

\indent $p \vee q$

\indent $(p \vee q) \cdot \sim (p \vee q)$

$\sim p$

\indent $q$

\indent $q \vee p$

\indent $p \vee q$

\indent $(p \vee q) \cdot \sim (p \vee q)$

$\sim q$

$\therefore \sim p \cdot \sim q$

\end{document}
